Clean up into_val injection

src/goose_lang/lib/into_val.v
@@ -4,7 +4,7 @@ From Perennial.goose_lang.lib Require Import typed_mem slice.slice struct.struct
 Class IntoVal {ext: ext_op} V :=
   { to_val: V -> val;
     IntoVal_def: V;
-    IntoVal_eq: ∀ v v', to_val v = to_val v' -> v = v'
+    IntoVal_inj :> Inj eq eq to_val;
   }.
 
 Class IntoValForType {ext V} (H: @IntoVal ext V) {ext_ty: ext_types ext} (t:ty) :=
@@ -13,58 +13,27 @@ Class IntoValForType {ext V} (H: @IntoVal ext V) {ext_ty: ext_types ext} (t:ty) 
       (* TODO: this isn't necessary, but it seems reasonable *)
       to_val_ty: forall v, val_ty (to_val v) t; }.
 
-Theorem IntoVal_eq_fmap_list {ext V} (H: @IntoVal ext V) :
-  ∀ (l l' : list V),
-  to_val <$> l = to_val <$> l' ->
-  l = l'.
+Instance Permutation_inj_list_fmap {A B} (f: A -> B) `{!Inj eq eq f} :
+  Inj (≡ₚ) (≡ₚ) (fmap (M:=list) f).
 Proof.
-  induction l; intros.
-  - destruct l'; simpl in *; congruence.
-  - destruct l'; simpl in *; try congruence.
-    inversion H0.
-    erewrite IHl; eauto.
-    eapply IntoVal_eq in H2; subst; eauto.
-Qed.
-
-Theorem IntoVal_eq_fmap_list_permutation {ext V} (H: @IntoVal ext V) :
-  ∀ (l l' : list V),
-  to_val <$> l ≡ₚ to_val <$> l' ->
-  l ≡ₚ l'.
-Proof.
-  induction l; intros.
-  - destruct l'; simpl in *; eauto.
-    exfalso. eapply Permutation_nil_cons. eauto.
-  - rewrite fmap_cons in H0. symmetry in H0.
-    eapply Permutation_cons_inv in H0.
-    destruct H0 as [l0' [l1' ?]]; intuition idtac.
-    eapply fmap_app_inv in H1.
-    destruct H1 as [l0 [l1 ?]]; intuition idtac. subst.
+  intros l.
+  induction l as [|x l IHl]; intros l' H.
+  - destruct l'; simpl in H; auto.
+    apply Permutation_nil_cons in H; contradiction.
+  - rewrite fmap_cons in H. symmetry in H.
+    eapply Permutation_cons_inv in H as (l0' & l1' & [Hfl Hfl']).
+    eapply fmap_app_inv in Hfl as (l0 & l1 & (->&Hfl&->)).
     destruct l1; first by simpl in *; congruence.
-    rewrite fmap_cons in H0. inversion H0; clear H0.
-    eapply IntoVal_eq in H3; subst.
+    rewrite fmap_cons in Hfl. inversion Hfl; clear Hfl.
+    apply (inj f) in H0; subst.
     eapply Permutation_cons_app.
     eapply IHl. rewrite fmap_app. eauto.
 Qed.
 
 Theorem IntoVal_eq_fmap_prod_permutation {ext V} (H: @IntoVal ext V) {K} :
-  ∀ (l l' : list (K * V)),
-  prod_map id to_val <$> l ≡ₚ prod_map id to_val <$> l' ->
-  l ≡ₚ l'.
+  Inj (≡ₚ) (≡ₚ) (fmap (prod_map (@id K) to_val)).
 Proof.
-  induction l; intros.
-  - destruct l'; simpl in *; eauto.
-    exfalso. eapply Permutation_nil_cons. eauto.
-  - rewrite fmap_cons in H0. symmetry in H0.
-    eapply Permutation_cons_inv in H0.
-    destruct H0 as [l0' [l1' ?]]; intuition idtac.
-    eapply fmap_app_inv in H1.
-    destruct H1 as [l0 [l1 ?]]; intuition idtac. subst.
-    destruct l1; first by simpl in *; congruence.
-    rewrite fmap_cons in H0. inversion H0; clear H0.
-    eapply IntoVal_eq in H4; subst.
-    destruct a, p; simpl in *; subst.
-    eapply Permutation_cons_app.
-    eapply IHl. rewrite fmap_app. eauto.
+  apply _.
 Qed.
 
 Theorem IntoVal_eq_fmap_map {ext V K} (H: @IntoVal ext V) `{Countable K}:
@@ -82,7 +51,7 @@ Proof.
   intros.
   eapply list_to_map_proper; eauto.
   rewrite -?list_to_map_fmap in H1.
-  eapply IntoVal_eq_fmap_prod_permutation.
+  apply (inj (fmap (prod_map id to_val))).
   eapply list_to_map_inj in H1; eauto.
   { rewrite -list_fmap_compose /compose /prod_map /=. eauto. }
   { rewrite -list_fmap_compose /compose /prod_map /=. eauto. }
@@ -91,31 +60,33 @@ Qed.
 (** instances for IntoVal *)
 Section instances.
   Context {ext: ext_op} {ext_ty: ext_types ext}.
-  Global Instance u64_IntoVal : IntoVal u64 :=
-    {| to_val := λ (x: u64), #x;
-       IntoVal_def := U64 0;
-       IntoVal_eq := ltac:(congruence) |}.
+  Global Instance u64_IntoVal : IntoVal u64.
+  Proof.
+    refine {| to_val := λ (x: u64), #x;
+              IntoVal_def := U64 0; |}; congruence.
+  Defined.
 
   Global Instance u64_IntoVal_uint64T : IntoValForType u64_IntoVal uint64T.
   Proof.
     constructor; auto.
   Qed.
 
-  Global Instance u8_IntoVal : IntoVal u8 :=
-    {| to_val := λ (x: u8), #x;
-       IntoVal_def := U8 0;
-       IntoVal_eq := ltac:(congruence) |}.
+  Global Instance u8_IntoVal : IntoVal u8.
+  Proof.
+    refine {| to_val := λ (x: u8), #x;
+              IntoVal_def := U8 0; |}; congruence.
+  Defined.
 
   Global Instance u8_IntoVal_byteT : IntoValForType u8_IntoVal byteT.
   Proof.
     constructor; eauto.
   Qed.
 
-  Global Instance loc_IntoVal : IntoVal loc :=
-    {| to_val := λ (l: loc), #l;
-       IntoVal_def := null;
-       IntoVal_eq := ltac:(congruence)
-    |}.
+  Global Instance loc_IntoVal : IntoVal loc.
+  Proof.
+    refine {| to_val := λ (l: loc), #l;
+              IntoVal_def := null; |}; congruence.
+  Defined.
 
   Global Instance loc_IntoVal_struct_ptr t : IntoValForType loc_IntoVal (struct.ptrT t).
   Proof.
@@ -131,11 +102,9 @@ Section instances.
     refine
     {| to_val := slice_val;
        IntoVal_def := Slice.nil;
-       IntoVal_eq := _
     |}.
-    destruct v, v'.
-    rewrite /slice_val /=.
-    intro H; inversion H; eauto.
+    intros [] [].
+    inversion 1; auto.
   Defined.
 
   Global Instance slice_IntoVal_ref t : IntoValForType slice_IntoVal (slice.T t).
